update MapBuiltinTypes with helper lemmas for seq/map

TypeInjections/TypeInjections.Test/Resources/MapBuiltinTypes.dfy
@@ -1,5 +1,6 @@
 module Translations.MapBuiltinTypes {
-
+    export reveals Seq, Set, Map
+    
     function Seq<o,n>(t: o -> n, e: seq<o>) : (f : seq<n>)
     ensures |e| == |f|
     ensures forall i : int :: (0 <= i < |e| ==> f[i] == t(e[i]))
@@ -7,27 +8,92 @@ module Translations.MapBuiltinTypes {
         if |e| == 0 then [] else
         seq(|e|, i => if 0 <= i < |e| then t(e[i]) else t(e[0]))
     }
-
     function Set<o,n>(t: o -> n, e: set<o>) : (f : set<n>)
     ensures forall x : o :: x in e ==> t(x) in f
     ensures forall x : n :: x in f ==> exists y : o :: y in e && t(y) == x
     {
         set x:o | x in e :: t(x)
     }
-
-    function Map<K_O,K_N,V_O,V_N>(K : K_O -> K_N, V : V_O -> V_N, e : map<K_O,V_O>) : (f: map<K_N,V_N>)
-    //ensures |e.Keys| == |f.Keys|
-    ensures forall x : K_N, y : V_N :: x in f.Keys && y in f.Values && f[x] == y 
-        ==> (exists a : K_O, b : V_O :: a in e.Keys && e[a] == b && K(a) == x && V(b) == y)
-    //ensures forall a : K_O, b : V_O :: a in e.Keys && b in e.Values && e[a] == b 
-    //    ==> (exists x : K_N, y : V_N :: x in f.Keys && y in f.Values && f[x] == y && K(a) == x && V(b) == y)    
+    function Map<K_O,K_N,V_O,V_N>(K : K_O -> K_N, V : V_O -> V_N, e : map<K_O,V_O>) : (f: map<K_N,V_N>)   
     {
         var fKeys := set x: K_O | x in e.Keys :: K(x);
         var fSet := set x:K_O | x in e.Keys :: (K(x),V(e[x]));
         map a | a in fKeys :: var b :| (a,b) in fSet; b
     }
-
-
+    /* Map helper functions and lemmas -- for proving map size meets standard of map31 */
+    function fKeysFunc<T_O(!new), T_N>(T: T_O->T_N, m_O: set<T_O>) : set<T_N>
+    {
+        set x: T_O | x in m_O :: T(x)
+    }
+    function fSetFunc<T_O(!new), T_N, U_O, U_N>(T: T_O->T_N, U: U_O->U_N, m_O: map<T_O,U_O>) : (res : set<(T_N,U_N)>)
+    {
+        var fKeys := fKeysFunc(T,m_O.Keys);
+        set x:T_O | x in m_O.Keys :: (T(x),U(m_O[x]))
+    }
+    function fMapFunc<T_O(!new), T_N, U_O, U_N>(T: T_O->T_N, U: U_O->U_N, m_O: map<T_O,U_O>) : (res : map<T_N,U_N>)
+    {
+        var fKeys := fKeysFunc(T,m_O.Keys);
+        var fSet := fSetFunc(T,U,m_O);
+        map a | a in fKeys :: var b :| (a,b) in fSet; b 
+    }
+    lemma testfKeysSize<T_O(!new), T_N>(T: T_O->T_N, m_O: set<T_O>)
+    requires forall x : T_O :: !exists y : T_O :: x != y && T(x) == T(y) 
+    ensures |fKeysFunc(T,m_O)| == |m_O|
+    {
+        var fKeys := fKeysFunc(T,m_O);
+        if |m_O| == 0 {
+            assert |fKeysFunc(T,m_O)| == |m_O|;
+        } else {
+            var x :| x in m_O;
+            var smallKeys := m_O - {x};
+            var fSmallKeys := fKeysFunc(T,smallKeys);
+            assert fKeys == fSmallKeys + {T(x)};
+            assert |fKeys| == |fSmallKeys| + 1;
+            testfKeysSize(T,smallKeys);
+        }
+    }
+    lemma testMapSize<T_O(!new), T_N, U_O, U_N>(T: T_O->T_N, U: U_O->U_N, m_O: map<T_O,U_O>)
+    requires forall x : T_O :: !exists y : T_O :: x != y && T(x) == T(y) 
+    ensures |fMapFunc(T,U,m_O).Keys| == |m_O.Keys|;
+    {
+        var fKeys := fKeysFunc(T,m_O.Keys);
+        testfKeysSize(T,m_O.Keys);
+        assert |fKeys| == |m_O.Keys|;
+        var fSet := fSetFunc(T,U,m_O);
+        var fMap := map a | a in fKeys :: var b :| (a,b) in fSet; b ;
+        if |m_O| == 0 {
+            assert |fMap.Keys| == |m_O.Keys|;
+        } else {
+            var x :| x in fKeys;
+            var smallKeys := fKeys - {x};
+            var fMapSmall := map a | a in smallKeys :: var b :| (a,b) in fSet; b;
+            assert fMap.Keys == fKeys;
+            assert |fMap.Keys| == |fKeys|;
+        }
+    }
+    function mapCreateGeneric<T_O(!new), T_N, U_O, U_N>(T: T_O->T_N, U: U_O->U_N, m_O: map<T_O,U_O>) : (res : map<T_N,U_N>)
+    requires forall x : T_O :: !exists y : T_O :: x != y && T(x) == T(y)
+    ensures forall x :: x in m_O.Keys ==> T(x) in res.Keys
+    ensures forall y :: y in m_O.Values ==> U(y) in res.Values
+    ensures |m_O.Keys| == |res.Keys|
+    {
+        testfKeysSize(T,m_O.Keys);
+        var fKeys := fKeysFunc(T,m_O.Keys);
+        var fSet := fSetFunc(T,U,m_O);
+        testMapSize(T,U,m_O);
+        map a | a in fKeys :: var b :| (a,b) in fSet; b 
+    }
+    /* Set helper functions and lemmas -- for proving set size meets standard of set31 */
+    function setCreate2Generic<o,n>(P : o -> n, S : set<o>) : set<n> 
+    { set x: o | x in S :: P(x) }
+    lemma setCreateSizeGeneric<o,n>(P : o -> n, S : set<o>)
+    ensures |setCreate2Generic(P,S)| <= |S|
+    {
+        if |S| == 0 { 
+        } else {
+            var x: o :| x in S;
+            assert setCreate2Generic(P,S) == setCreate2Generic(P,S - {x}) + {P(x)};
+            setCreateSizeGeneric(P,S - {x});
+        }
+    }
 }
-
-
